\section{Задача 1.25}
\subsection{Задание:}
Найти матрицу обратную к
$
	A =
	\begin{pmatrix}
		2 & 4 & 0 & 1 \\
		3 & -3 & 5 & 0 \\
		-1 & 0 & 1 & 1 \\
		2 & 1 & 1 & 0 \\
	\end{pmatrix}
$
\; методом алгебраических дополненй.
\subsection{Решение:}
Найдём $ \det A $ чтобы убедиться что $ \exists A^{-1} $:
\\[1em]
$
	\det A =
	\begin{vmatrix}
		2 & 4 & 0 & 1 \\
		3 & -3 & 5 & 0 \\
		-1 & 0 & 1 & 1 \\
		2 & 1 & 1 & 0 \\
	\end{vmatrix}
	=
	\begin{vmatrix}
		3 & 4 & -1 & 0 \\
		3 & -3 & 5 & 0 \\
		-1 & 0 & 1 & 1 \\
		2 & 1 & 1 & 0 \\
	\end{vmatrix}
	=
	\begin{vmatrix}
		3 & 4 & -1 & 0 \\
		3 & -3 & 5 & 0 \\
		-1 & 0 & 1 & 1 \\
		2 & 1 & 1 & 0 \\
	\end{vmatrix}
	=
	-
	\begin{vmatrix}
		3 & 4 & -1 \\
		3 & -3 & 5 \\
		2 & 1 & 1 \\
	\end{vmatrix}
	=
	5
$
\\[1em]
$ \det A \neq 0 \Rightarrow \exists A^{-1} = \dfrac{D^T}{\det A} $
\\[1em]
$
	d_{11} =
	\begin{vmatrix}
		-3 & 5 & 0 \\
		0 & 1 & 1 \\
		1 & 1 & 0 \\
	\end{vmatrix}
	=
	\begin{vmatrix}
		-3 & 5 & 0 \\
		0 & 1 & 1 \\
		1 & 1 & 0 \\
	\end{vmatrix}
	=
	-
	\begin{vmatrix}
		-3 & 5 \\
		1 & 1 \\
	\end{vmatrix}
	= 8
\\[1em]
	d_{12} =
	\begin{vmatrix}
		3 & 5 & 0 \\
		-1 & 1 & 1 \\
		2 & 1 & 0 \\
	\end{vmatrix}
	=
	-
	\begin{vmatrix}
		3 & 5 \\
		2 & 1 \\
	\end{vmatrix}
	=
	7
\\[1em]
	d_{13} =
	\begin{vmatrix}
		3 & -3 & 0 \\
		-1 & 0 & 1 \\
		2 & 1 & 0 \\
	\end{vmatrix}
	=
	-
	\begin{vmatrix}
		3 & -3 \\
		2 & 1 \\
	\end{vmatrix}
	=
	-9
\\[1em]
	d_{14} =
	\begin{vmatrix}
		3 & -3 & 5 \\
		-1 & 0 & 1 \\
		2 & 1 & 1 \\
	\end{vmatrix}
	=
	\begin{vmatrix}
		-3 & 5 \\
		1 & 1 \\
	\end{vmatrix}
	-
	\begin{vmatrix}
		3 & -3 \\
		2 & 1 \\
	\end{vmatrix}
	=
	-8 - 9 = -17
\\[1em]
	d_{21} =
	\begin{vmatrix}
		4 & 0 & 1 \\
		0 & 1 & 1 \\
		1 & 1 & 0 \\
	\end{vmatrix}
	=
	4
	\begin{vmatrix}
		1 & 1 \\
		1 & 0
	\end{vmatrix}
	+
	\begin{vmatrix}
		0 & 1 \\
		1 & 1
	\end{vmatrix}
	= -4 - 1 = -5
\\[1em]
	d_{22} =
	\begin{vmatrix}
		2  & 0 & 1 \\
		-1 & 1 & 1 \\
		2 & 1 & 0 \\
	\end{vmatrix}
	=
	2
	\begin{vmatrix}
		1 & 1 \\
		1 & 0 \\
	\end{vmatrix}
	+
	\begin{vmatrix}
		-1 & 1 \\
		2 & 1 \\
	\end{vmatrix}
	= -2 - 3 = -5
\\[1em]
$
